<?xml version="1.0" encoding="UTF-8"?>
<!DOCTYPE rdf:RDF [
    <!ENTITY rdfns 'http://www.w3.org/1999/02/22-rdf-syntax-ns#'>
    <!ENTITY rdfsns 'http://www.w3.org/2000/01/rdf-schema#'>
    <!ENTITY dcns 'http://purl.org/dc/elements/1.1/'>
    <!ENTITY dctermsns 'http://purl.org/dc/terms/'>
    <!ENTITY dctypens 'http://purl.org/dc/dcmitype/'>
]>
<rdf:RDF xmlns:rdf="http://www.w3.org/1999/02/22-rdf-syntax-ns#" xmlns:dcterms="http://purl.org/dc/terms/" xmlns:dc="http://purl.org/dc/elements/1.1/" xmlns:rdfs="http://www.w3.org/2000/01/rdf-schema#">
<rdf:Description rdf:about="http://purl.org/dc/terms/">
<dc:title>The Dublin Core Terms Namespace providing access to its content by means of an RDF Schema.</dc:title>
<dc:publisher>The Dublin Core Metadata Initiative</dc:publisher>
<dc:description>The Dublin Core Terms namespace provides URIs for the Dublin Core Element Set Qualifier Vocabulary. Vocabulary terms are declared using RDF Schema language to support RDF applications. The Dublin Core qualifiers form a richer vocabulary, which is intended to facilitate discovery of resources. It will be updated according to dc-usage decisions.</dc:description>
<dc:language>English</dc:language>
<dcterms:issued>2000-07-11</dcterms:issued>
<dcterms:modified>2002-05-24</dcterms:modified>
<dc:source rdf:resource="http://www.dublincore.org/documents/2000/07/11/dcmes-qualifiers/"/>
<dc:source rdf:resource="http://www.dublincore.org/usage/decisions/"/>
<dcterms:requires rdf:resource="http://purl.org/dc/elements/1.1/"/>
<dcterms:references rdf:resource="http://purl.org/dc/dcmitype/"/>
</rdf:Description>
<rdf:Property rdf:about="http://purl.org/dc/terms/audience">
<rdfs:label>Audience</rdfs:label>
<rdfs:comment>A class of entity for whom the resource is intended or useful.</rdfs:comment>
<dc:description>A class of entity may be determined by the creator or the 
		publisher or by a third party.</dc:description>
<rdfs:isDefinedBy rdf:resource="http://purl.org/dc/terms/"/>
<dcterms:issued>2001-05-21</dcterms:issued>
<dcterms:modified>2002-06-15</dcterms:modified>
<dc:type rdf:resource="http://dublincore.org/usage/documents/principles/#element"/>
<dcterms:hasVersion rdf:resource="http://dublincore.org/usage/terms/history/#audience-002"/>
</rdf:Property>
<rdf:Property rdf:about="http://purl.org/dc/terms/alternative">
<rdfs:label>Alternative</rdfs:label>
<rdfs:comment>Any form of the title used as a substitute or alternative 
		to the formal title of the resource.</rdfs:comment>
<dc:description>This qualifier can include Title abbreviations as well 
		as translations.</dc:description>
<rdfs:isDefinedBy rdf:resource="http://purl.org/dc/terms/"/>
<dcterms:issued>2000-07-11</dcterms:issued>
<dcterms:modified>2002-06-15</dcterms:modified>
<rdfs:subPropertyOf rdf:resource="http://purl.org/dc/elements/1.1/title"/>
<dc:type rdf:resource="http://dublincore.org/usage/documents/principles/#element-refinement"/>
<dcterms:hasVersion rdf:resource="http://dublincore.org/usage/terms/history/#alternative-002"/>
</rdf:Property>
<rdf:Property rdf:about="http://purl.org/dc/terms/tableOfContents">
<rdfs:label>Table Of Contents</rdfs:label>
<rdfs:comment>A list of subunits of the content of the resource.</rdfs:comment>
<rdfs:isDefinedBy rdf:resource="http://purl.org/dc/terms/"/>
<dcterms:issued>2000-07-11</dcterms:issued>
<dcterms:modified>2002-06-15</dcterms:modified>
<rdfs:subPropertyOf rdf:resource="http://purl.org/dc/elements/1.1/description"/>
<dc:type rdf:resource="http://dublincore.org/usage/documents/principles/#element-refinement"/>
<dcterms:hasVersion rdf:resource="http://dublincore.org/usage/terms/history/#tableOfContents-002"/>
</rdf:Property>
<rdf:Property rdf:about="http://purl.org/dc/terms/abstract">
<rdfs:label>Abstract</rdfs:label>
<rdfs:comment>A summary of the content of the resource.</rdfs:comment>
<rdfs:isDefinedBy rdf:resource="http://purl.org/dc/terms/"/>
<dcterms:issued>2000-07-11</dcterms:issued>
<dcterms:modified>2002-06-15</dcterms:modified>
<rdfs:subPropertyOf rdf:resource="http://purl.org/dc/elements/1.1/description"/>
<dc:type rdf:resource="http://dublincore.org/usage/documents/principles/#element-refinement"/>
<dcterms:hasVersion rdf:resource="http://dublincore.org/usage/terms/history/#abstract-002"/>
</rdf:Property>
<rdf:Property rdf:about="http://purl.org/dc/terms/created">
<rdfs:label>Created</rdfs:label>
<rdfs:comment>Date of creation of the resource.</rdfs:comment>
<rdfs:isDefinedBy rdf:resource="http://purl.org/dc/terms/"/>
<dcterms:issued>2000-07-11</dcterms:issued>
<dcterms:modified>2002-06-15</dcterms:modified>
<rdfs:subPropertyOf rdf:resource="http://purl.org/dc/elements/1.1/date"/>
<dc:type rdf:resource="http://dublincore.org/usage/documents/principles/#element-refinement"/>
<dcterms:hasVersion rdf:resource="http://dublincore.org/usage/terms/history/#created-002"/>
</rdf:Property>
<rdf:Property rdf:about="http://purl.org/dc/terms/valid">
<rdfs:label>Valid</rdfs:label>
<rdfs:comment>Date (often a range) of validity of a resource.</rdfs:comment>
<rdfs:isDefinedBy rdf:resource="http://purl.org/dc/terms/"/>
<dcterms:issued>2000-07-11</dcterms:issued>
<dcterms:modified>2002-06-15</dcterms:modified>
<rdfs:subPropertyOf rdf:resource="http://purl.org/dc/elements/1.1/date"/>
<dc:type rdf:resource="http://dublincore.org/usage/documents/principles/#element-refinement"/>
<dcterms:hasVersion rdf:resource="http://dublincore.org/usage/terms/history/#valid-002"/>
</rdf:Property>
<rdf:Property rdf:about="http://purl.org/dc/terms/available">
<rdfs:label>Available</rdfs:label>
<rdfs:comment>Date (often a range) that the resource will become or did 
		become available.</rdfs:comment>
<rdfs:isDefinedBy rdf:resource="http://purl.org/dc/terms/"/>
<dcterms:issued>2000-07-11</dcterms:issued>
<dcterms:modified>2002-06-15</dcterms:modified>
<rdfs:subPropertyOf rdf:resource="http://purl.org/dc/elements/1.1/date"/>
<dc:type rdf:resource="http://dublincore.org/usage/documents/principles/#element-refinement"/>
<dcterms:hasVersion rdf:resource="http://dublincore.org/usage/terms/history/#available-002"/>
</rdf:Property>
<rdf:Property rdf:about="http://purl.org/dc/terms/issued">
<rdfs:label>Issued</rdfs:label>
<rdfs:comment>Date of formal issuance (e.g., publication) of the resource.</rdfs:comment>
<rdfs:isDefinedBy rdf:resource="http://purl.org/dc/terms/"/>
<dcterms:issued>2000-07-11</dcterms:issued>
<dcterms:modified>2002-06-15</dcterms:modified>
<rdfs:subPropertyOf rdf:resource="http://purl.org/dc/elements/1.1/date"/>
<dc:type rdf:resource="http://dublincore.org/usage/documents/principles/#element-refinement"/>
<dcterms:hasVersion rdf:resource="http://dublincore.org/usage/terms/history/#issued-002"/>
</rdf:Property>
<rdf:Property rdf:about="http://purl.org/dc/terms/modified">
<rdfs:label>Modified</rdfs:label>
<rdfs:comment>Date on which the resource was changed.</rdfs:comment>
<rdfs:isDefinedBy rdf:resource="http://purl.org/dc/terms/"/>
<dcterms:issued>2000-07-11</dcterms:issued>
<dcterms:modified>2002-06-15</dcterms:modified>
<rdfs:subPropertyOf rdf:resource="http://purl.org/dc/elements/1.1/date"/>
<dc:type rdf:resource="http://dublincore.org/usage/documents/principles/#element-refinement"/>
<dcterms:hasVersion rdf:resource="http://dublincore.org/usage/terms/history/#modified-002"/>
</rdf:Property>
<rdf:Property rdf:about="http://purl.org/dc/terms/extent">
<rdfs:label>Extent</rdfs:label>
<rdfs:comment>The size or duration of the resource.</rdfs:comment>
<rdfs:isDefinedBy rdf:resource="http://purl.org/dc/terms/"/>
<dcterms:issued>2000-07-11</dcterms:issued>
<dcterms:modified>2002-06-15</dcterms:modified>
<rdfs:subPropertyOf rdf:resource="http://purl.org/dc/elements/1.1/format"/>
<dc:type rdf:resource="http://dublincore.org/usage/documents/principles/#element-refinement"/>
<dcterms:hasVersion rdf:resource="http://dublincore.org/usage/terms/history/#extent-002"/>
</rdf:Property>
<rdf:Property rdf:about="http://purl.org/dc/terms/medium">
<rdfs:label>Medium</rdfs:label>
<rdfs:comment>The material or physical carrier of the resource.</rdfs:comment>
<rdfs:isDefinedBy rdf:resource="http://purl.org/dc/terms/"/>
<dcterms:issued>2000-07-11</dcterms:issued>
<dcterms:modified>2002-06-15</dcterms:modified>
<rdfs:subPropertyOf rdf:resource="http://purl.org/dc/elements/1.1/format"/>
<dc:type rdf:resource="http://dublincore.org/usage/documents/principles/#element-refinement"/>
<dcterms:hasVersion rdf:resource="http://dublincore.org/usage/terms/history/#medium-002"/>
</rdf:Property>
<rdf:Property rdf:about="http://purl.org/dc/terms/isVersionOf">
<rdfs:label>Is Version Of</rdfs:label>
<rdfs:comment>The described resource is a version, edition, or adaptation 
		of the referenced resource. Changes in version imply substantive 
		changes in content rather than differences in format.</rdfs:comment>
<rdfs:isDefinedBy rdf:resource="http://purl.org/dc/terms/"/>
<dcterms:issued>2000-07-11</dcterms:issued>
<dcterms:modified>2002-06-15</dcterms:modified>
<rdfs:subPropertyOf rdf:resource="http://purl.org/dc/elements/1.1/relation"/>
<dc:type rdf:resource="http://dublincore.org/usage/documents/principles/#element-refinement"/>
<dcterms:hasVersion rdf:resource="http://dublincore.org/usage/terms/history/#isVersionOf-002"/>
</rdf:Property>
<rdf:Property rdf:about="http://purl.org/dc/terms/hasVersion">
<rdfs:label>Has Version</rdfs:label>
<rdfs:comment>The described resource has a version, edition, or adaptation, 
		namely, the referenced resource.</rdfs:comment>
<rdfs:isDefinedBy rdf:resource="http://purl.org/dc/terms/"/>
<dcterms:issued>2000-07-11</dcterms:issued>
<dcterms:modified>2002-06-15</dcterms:modified>
<rdfs:subPropertyOf rdf:resource="http://purl.org/dc/elements/1.1/relation"/>
<dc:type rdf:resource="http://dublincore.org/usage/documents/principles/#element-refinement"/>
<dcterms:hasVersion rdf:resource="http://dublincore.org/usage/terms/history/#hasVersion-002"/>
</rdf:Property>
<rdf:Property rdf:about="http://purl.org/dc/terms/isReplacedBy">
<rdfs:label>Is Replaced By</rdfs:label>
<rdfs:comment>The described resource is supplanted, displaced, or 
		superseded by the referenced resource.</rdfs:comment>
<rdfs:isDefinedBy rdf:resource="http://purl.org/dc/terms/"/>
<dcterms:issued>2000-07-11</dcterms:issued>
<dcterms:modified>2002-06-15</dcterms:modified>
<rdfs:subPropertyOf rdf:resource="http://purl.org/dc/elements/1.1/relation"/>
<dc:type rdf:resource="http://dublincore.org/usage/documents/principles/#element-refinement"/>
<dcterms:hasVersion rdf:resource="http://dublincore.org/usage/terms/history/#isReplacedBy-002"/>
</rdf:Property>
<rdf:Property rdf:about="http://purl.org/dc/terms/replaces">
<rdfs:label>Replaces</rdfs:label>
<rdfs:comment>The described resource supplants, displaces, or supersedes 
		the referenced resource.</rdfs:comment>
<rdfs:isDefinedBy rdf:resource="http://purl.org/dc/terms/"/>
<dcterms:issued>2000-07-11</dcterms:issued>
<dcterms:modified>2002-06-15</dcterms:modified>
<rdfs:subPropertyOf rdf:resource="http://purl.org/dc/elements/1.1/relation"/>
<dc:type rdf:resource="http://dublincore.org/usage/documents/principles/#element-refinement"/>
<dcterms:hasVersion rdf:resource="http://dublincore.org/usage/terms/history/#replaces-002"/>
</rdf:Property>
<rdf:Property rdf:about="http://purl.org/dc/terms/isRequiredBy">
<rdfs:label>Is Required By</rdfs:label>
<rdfs:comment>The described resource is required by the referenced resource, 
		either physically or logically.</rdfs:comment>
<rdfs:isDefinedBy rdf:resource="http://purl.org/dc/terms/"/>
<dcterms:issued>2000-07-11</dcterms:issued>
<dcterms:modified>2002-06-15</dcterms:modified>
<rdfs:subPropertyOf rdf:resource="http://purl.org/dc/elements/1.1/relation"/>
<dc:type rdf:resource="http://dublincore.org/usage/documents/principles/#element-refinement"/>
<dcterms:hasVersion rdf:resource="http://dublincore.org/usage/terms/history/#isRequiredBy-002"/>
</rdf:Property>
<rdf:Property rdf:about="http://purl.org/dc/terms/requires">
<rdfs:label>Requires</rdfs:label>
<rdfs:comment>The described resource requires the referenced resource to 
		support its function, delivery, or coherence of content.</rdfs:comment>
<rdfs:isDefinedBy rdf:resource="http://purl.org/dc/terms/"/>
<dcterms:issued>2000-07-11</dcterms:issued>
<dcterms:modified>2002-06-15</dcterms:modified>
<rdfs:subPropertyOf rdf:resource="http://purl.org/dc/elements/1.1/relation"/>
<dc:type rdf:resource="http://dublincore.org/usage/documents/principles/#element-refinement"/>
<dcterms:hasVersion rdf:resource="http://dublincore.org/usage/terms/history/#requires-002"/>
</rdf:Property>
<rdf:Property rdf:about="http://purl.org/dc/terms/isPartOf">
<rdfs:label>Is Part Of</rdfs:label>
<rdfs:comment>The described resource is a physical or logical part of the 
		referenced resource.</rdfs:comment>
<rdfs:isDefinedBy rdf:resource="http://purl.org/dc/terms/"/>
<dcterms:issued>2000-07-11</dcterms:issued>
<dcterms:modified>2002-06-15</dcterms:modified>
<rdfs:subPropertyOf rdf:resource="http://purl.org/dc/elements/1.1/relation"/>
<dc:type rdf:resource="http://dublincore.org/usage/documents/principles/#element-refinement"/>
<dcterms:hasVersion rdf:resource="http://dublincore.org/usage/terms/history/#isPartOf-002"/>
</rdf:Property>
<rdf:Property rdf:about="http://purl.org/dc/terms/hasPart">
<rdfs:label>Has Part</rdfs:label>
<rdfs:comment>The described resource includes the referenced resource either 
		physically or logically.</rdfs:comment>
<rdfs:isDefinedBy rdf:resource="http://purl.org/dc/terms/"/>
<dcterms:issued>2000-07-11</dcterms:issued>
<dcterms:modified>2002-06-15</dcterms:modified>
<rdfs:subPropertyOf rdf:resource="http://purl.org/dc/elements/1.1/relation"/>
<dc:type rdf:resource="http://dublincore.org/usage/documents/principles/#element-refinement"/>
<dcterms:hasVersion rdf:resource="http://dublincore.org/usage/terms/history/#hasPart-002"/>
</rdf:Property>
<rdf:Property rdf:about="http://purl.org/dc/terms/isReferencedBy">
<rdfs:label>Is Referenced By</rdfs:label>
<rdfs:comment>The described resource is referenced, cited, or otherwise 
		pointed to by the referenced resource.</rdfs:comment>
<rdfs:isDefinedBy rdf:resource="http://purl.org/dc/terms/"/>
<dcterms:issued>2000-07-11</dcterms:issued>
<dcterms:modified>2002-06-15</dcterms:modified>
<rdfs:subPropertyOf rdf:resource="http://purl.org/dc/elements/1.1/relation"/>
<dc:type rdf:resource="http://dublincore.org/usage/documents/principles/#element-refinement"/>
<dcterms:hasVersion rdf:resource="http://dublincore.org/usage/terms/history/#isReferencedBy-002"/>
</rdf:Property>
<rdf:Property rdf:about="http://purl.org/dc/terms/references">
<rdfs:label>References</rdfs:label>
<rdfs:comment>The described resource references, cites, or otherwise points 
		to the referenced resource.</rdfs:comment>
<rdfs:isDefinedBy rdf:resource="http://purl.org/dc/terms/"/>
<dcterms:issued>2000-07-11</dcterms:issued>
<dcterms:modified>2002-06-15</dcterms:modified>
<rdfs:subPropertyOf rdf:resource="http://purl.org/dc/elements/1.1/relation"/>
<dc:type rdf:resource="http://dublincore.org/usage/documents/principles/#element-refinement"/>
<dcterms:hasVersion rdf:resource="http://dublincore.org/usage/terms/history/#references-002"/>
</rdf:Property>
<rdf:Property rdf:about="http://purl.org/dc/terms/isFormatOf">
<rdfs:label>Is Format Of</rdfs:label>
<rdfs:comment>The described resource is the same intellectual content of 
		the referenced resource, but presented in another format.</rdfs:comment>
<rdfs:isDefinedBy rdf:resource="http://purl.org/dc/terms/"/>
<dcterms:issued>2000-07-11</dcterms:issued>
<dcterms:modified>2002-06-15</dcterms:modified>
<rdfs:subPropertyOf rdf:resource="http://purl.org/dc/elements/1.1/relation"/>
<dc:type rdf:resource="http://dublincore.org/usage/documents/principles/#element-refinement"/>
<dcterms:hasVersion rdf:resource="http://dublincore.org/usage/terms/history/#isFormatOf-002"/>
</rdf:Property>
<rdf:Property rdf:about="http://purl.org/dc/terms/hasFormat">
<rdfs:label>Has Format</rdfs:label>
<rdfs:comment>The described resource pre-existed the referenced resource, 
		which is essentially the same intellectual content presented 
		in another format.</rdfs:comment>
<rdfs:isDefinedBy rdf:resource="http://purl.org/dc/terms/"/>
<dcterms:issued>2000-07-11</dcterms:issued>
<dcterms:modified>2002-06-15</dcterms:modified>
<rdfs:subPropertyOf rdf:resource="http://purl.org/dc/elements/1.1/relation"/>
<dc:type rdf:resource="http://dublincore.org/usage/documents/principles/#element-refinement"/>
<dcterms:hasVersion rdf:resource="http://dublincore.org/usage/terms/history/#hasFormat-002"/>
</rdf:Property>
<rdf:Property rdf:about="http://purl.org/dc/terms/conformsTo">
<rdfs:label>Conforms To</rdfs:label>
<rdfs:comment>A reference to an established standard to which the resource conforms.</rdfs:comment>
<rdfs:isDefinedBy rdf:resource="http://purl.org/dc/terms/"/>
<dcterms:issued>2001-05-21</dcterms:issued>
<dcterms:modified>2002-06-15</dcterms:modified>
<rdfs:subPropertyOf rdf:resource="http://purl.org/dc/elements/1.1/relation"/>
<dc:type rdf:resource="http://dublincore.org/usage/documents/principles/#element-refinement"/>
<dcterms:hasVersion rdf:resource="http://dublincore.org/usage/terms/history/#conformsTo-002"/>
</rdf:Property>
<rdf:Property rdf:about="http://purl.org/dc/terms/spatial">
<rdfs:label>Spatial</rdfs:label>
<rdfs:comment>Spatial characteristics of the intellectual content of the resource.</rdfs:comment>
<rdfs:isDefinedBy rdf:resource="http://purl.org/dc/terms/"/>
<dcterms:issued>2000-07-11</dcterms:issued>
<dcterms:modified>2002-06-15</dcterms:modified>
<rdfs:subPropertyOf rdf:resource="http://purl.org/dc/elements/1.1/coverage"/>
<dc:type rdf:resource="http://dublincore.org/usage/documents/principles/#element-refinement"/>
<dcterms:hasVersion rdf:resource="http://dublincore.org/usage/terms/history/#spatial-002"/>
</rdf:Property>
<rdf:Property rdf:about="http://purl.org/dc/terms/temporal">
<rdfs:label>Temporal</rdfs:label>
<rdfs:comment>Temporal characteristics of the intellectual content of the resource.</rdfs:comment>
<rdfs:isDefinedBy rdf:resource="http://purl.org/dc/terms/"/>
<dcterms:issued>2000-07-11</dcterms:issued>
<dcterms:modified>2002-06-15</dcterms:modified>
<rdfs:subPropertyOf rdf:resource="http://purl.org/dc/elements/1.1/coverage"/>
<dc:type rdf:resource="http://dublincore.org/usage/documents/principles/#element-refinement"/>
<dcterms:hasVersion rdf:resource="http://dublincore.org/usage/terms/history/#temporal-002"/>
</rdf:Property>
<rdf:Property rdf:about="http://purl.org/dc/terms/mediator">
<rdfs:label>Mediator</rdfs:label>
<rdfs:comment>A class of entity that mediates access to the
		resource and for whom the resource is intended or useful.</rdfs:comment>
<dc:description>The audiences for a resource are of two basic classes: (1) an 
		ultimate beneficiary of the resource, and (2) frequently, an 
		entity that mediates access to the resource.  The mediator 
		element refinement represents the second of these two classes.</dc:description>
<rdfs:isDefinedBy rdf:resource="http://purl.org/dc/terms/"/>
<dcterms:issued>2001-05-21</dcterms:issued>
<dcterms:modified>2002-07-13</dcterms:modified>
<rdfs:subPropertyOf rdf:resource="http://purl.org/dc/terms/audience"/>
<dc:type rdf:resource="http://dublincore.org/usage/documents/principles/#element-refinement"/>
<dcterms:hasVersion rdf:resource="http://dublincore.org/usage/terms/history/#mediator-002"/>
</rdf:Property>
<rdf:Property rdf:about="http://purl.org/dc/terms/dateAccepted">
<rdfs:label>Date Accepted</rdfs:label>
<rdfs:comment>Date of acceptance of the resource (e.g. of thesis
		by university department, of article by journal, etc.).</rdfs:comment>
<rdfs:isDefinedBy rdf:resource="http://purl.org/dc/terms/"/>
<dcterms:issued>2002-07-13</dcterms:issued>
<rdfs:subPropertyOf rdf:resource="http://purl.org/dc/elements/1.1/date"/>
<dc:type rdf:resource="http://dublincore.org/usage/documents/principles/#element-refinement"/>
<dcterms:hasVersion rdf:resource="http://dublincore.org/usage/terms/history/#dateAccepted-001"/>
</rdf:Property>
<rdf:Property rdf:about="http://purl.org/dc/terms/dateCopyrighted">
<rdfs:label>Date Copyrighted</rdfs:label>
<rdfs:comment>Date of a statement of copyright.</rdfs:comment>
<rdfs:isDefinedBy rdf:resource="http://purl.org/dc/terms/"/>
<dcterms:issued>2002-07-13</dcterms:issued>
<rdfs:subPropertyOf rdf:resource="http://purl.org/dc/elements/1.1/date"/>
<dc:type rdf:resource="http://dublincore.org/usage/documents/principles/#element-refinement"/>
<dcterms:hasVersion rdf:resource="http://dublincore.org/usage/terms/history/#dateCopyrighted-001"/>
</rdf:Property>
<rdf:Property rdf:about="http://purl.org/dc/terms/dateSubmitted">
<rdfs:label>Date Submitted</rdfs:label>
<rdfs:comment>Date of submission of the resource (e.g. thesis, 
		articles, etc.).</rdfs:comment>
<rdfs:isDefinedBy rdf:resource="http://purl.org/dc/terms/"/>
<dcterms:issued>2002-07-13</dcterms:issued>
<rdfs:subPropertyOf rdf:resource="http://purl.org/dc/elements/1.1/date"/>
<dc:type rdf:resource="http://dublincore.org/usage/documents/principles/#element-refinement"/>
<dcterms:hasVersion rdf:resource="http://dublincore.org/usage/terms/history/#dateSubmitted-001"/>
</rdf:Property>
<rdf:Property rdf:about="http://purl.org/dc/terms/educationLevel">
<rdfs:label>Audience Education Level</rdfs:label>
<rdfs:comment>A general statement describing the education or 
		training context.  Alternatively, a more specific 
		statement of the location of the audience in terms of 
		its progression through an education or training context.</rdfs:comment>
<rdfs:isDefinedBy rdf:resource="http://purl.org/dc/terms/"/>
<dcterms:issued>2002-07-13</dcterms:issued>
<rdfs:subPropertyOf rdf:resource="http://purl.org/dc/terms/audience"/>
<dc:type rdf:resource="http://dublincore.org/usage/documents/principles/#element-refinement"/>
<dcterms:hasVersion rdf:resource="http://dublincore.org/usage/terms/history/#educationLevel-001"/>
</rdf:Property>
<rdf:Property rdf:about="http://purl.org/dc/terms/accessRights">
<rdfs:label>Access Rights</rdfs:label>
<rdfs:comment>Information about who can access the
        resource or an indication of its security status.
        </rdfs:comment>
<dc:description>Access Rights may include information
        regarding access or restrictions based on privacy, 
        security or other regulations.
        </dc:description>
<rdfs:isDefinedBy rdf:resource="http://purl.org/dc/terms/"/>
<dcterms:issued>2003-02-15</dcterms:issued>
<rdfs:subPropertyOf rdf:resource="http://purl.org/dc/elements/1.1/rights"/>
<dc:type rdf:resource="http://dublincore.org/usage/documents/principles/#element-refinement"/>
<dcterms:hasVersion rdf:resource="http://dublincore.org/usage/terms/history/#accessRights-001"/>
</rdf:Property>
<rdf:Property rdf:about="http://purl.org/dc/terms/bibliographicCitation">
<rdfs:label>Bibliographic Citation</rdfs:label>
<rdfs:comment>A bibliographic reference for the resource.
        </rdfs:comment>
<dc:description>Recommended practice is to include sufficient 
        bibliographic detail to identify the resource as 
        unambiguously as possible, whether or not the
        citation is in a standard form.
        </dc:description>
<rdfs:isDefinedBy rdf:resource="http://purl.org/dc/terms/"/>
<dcterms:issued>2003-02-15</dcterms:issued>
<rdfs:subPropertyOf rdf:resource="http://purl.org/dc/elements/1.1/identifier"/>
<dc:type rdf:resource="http://dublincore.org/usage/documents/principles/#element-refinement"/>
<dcterms:hasVersion rdf:resource="http://dublincore.org/usage/terms/history/#bibliographicCitation-001"/>
</rdf:Property>
<rdf:Property rdf:about="http://purl.org/dc/terms/license">
<rdfs:label>License</rdfs:label>
<rdfs:comment>A legal document giving official permission to do something
        with the resource.</rdfs:comment>
<dc:description>Recommended best practice is to identify the license using a
        URI. Examples of such licenses can be found at
        http://creativecommons.org/licenses/.</dc:description>
<rdfs:isDefinedBy rdf:resource="http://purl.org/dc/terms/"/>
<dcterms:issued>2004-06-14</dcterms:issued>
<rdfs:subPropertyOf rdf:resource="http://purl.org/dc/elements/1.1/rights"/>
<dc:type rdf:resource="http://dublincore.org/usage/documents/principles/#element-refinement"/>
<dcterms:hasVersion rdf:resource="http://dublincore.org/usage/terms/history/#license-001"/>
</rdf:Property>
<rdf:Property rdf:about="http://purl.org/dc/terms/rightsHolder">
<rdfs:label>Rights Holder</rdfs:label>
<rdfs:comment>A person or organization owning or managing rights over the resource.
        </rdfs:comment>
<dc:description>Recommended best practice is to use the URI or name of
        the Rights Holder to indicate the entity.</dc:description>
<rdfs:isDefinedBy rdf:resource="http://purl.org/dc/terms/"/>
<dcterms:issued>2004-06-14</dcterms:issued>
<dc:type rdf:resource="http://dublincore.org/usage/documents/principles/#element"/>
<dcterms:hasVersion rdf:resource="http://dublincore.org/usage/terms/history/#rightsHolder-001"/>
</rdf:Property>
<rdf:Property rdf:about="http://purl.org/dc/terms/provenance">
<rdfs:label>Provenance</rdfs:label>
<rdfs:comment>A statement of any changes in ownership and custody
        of the resource since its creation that are
        significant for its authenticity, integrity and
        interpretation.
        </rdfs:comment>
<dc:description>The statement may include a description of any
        changes successive custodians made to the resource.
        </dc:description>
<rdfs:isDefinedBy rdf:resource="http://purl.org/dc/terms/"/>
<dcterms:issued>2004-09-20</dcterms:issued>
<dc:type rdf:resource="http://dublincore.org/usage/documents/principles/#element"/>
<dcterms:hasVersion rdf:resource="http://dublincore.org/usage/terms/history/#provenance-001"/>
</rdf:Property>
<rdf:Property rdf:about="http://purl.org/dc/terms/instructionalMethod">
<rdfs:label>Instructional Method</rdfs:label>
<rdfs:comment>A process, used to engender knowledge, attitudes and skills,
                    that the resource is designed to support.</rdfs:comment>
<dc:description>Instructional Method will typically include ways of presenting
                 instructional materials or conducting instructional activities,
                 patterns of learner-to-learner and learner-to-instructor interactions,
                 and mechanisms by which group and individual levels of learning are measured.
                 Instructional methods include all aspects of the instruction and learning
                 processes from planning and implementation through evaluation and 
                 feedback.</dc:description>
<rdfs:isDefinedBy rdf:resource="http://purl.org/dc/terms/"/>
<dcterms:issued>2005-06-13</dcterms:issued>
<dc:type rdf:resource="http://dublincore.org/usage/documents/principles/#element"/>
<dcterms:hasVersion rdf:resource="http://dublincore.org/usage/terms/history/#instructionalMethod-001"/>
</rdf:Property>
<rdf:Property rdf:about="http://purl.org/dc/terms/accrualMethod">
<rdfs:label>Accrual Method</rdfs:label>
<rdfs:comment>The method by which items are added to a collection.</rdfs:comment>
<dc:description>Recommended best practice is to use a value from a controlled
                 vocabulary.</dc:description>
<rdfs:isDefinedBy rdf:resource="http://purl.org/dc/terms/"/>
<dcterms:issued>2005-06-13</dcterms:issued>
<dc:type rdf:resource="http://dublincore.org/usage/documents/principles/#element"/>
<dcterms:hasVersion rdf:resource="http://dublincore.org/usage/terms/history/#accrualMethod-001"/>
</rdf:Property>
<rdf:Property rdf:about="http://purl.org/dc/terms/accrualPeriodicity">
<rdfs:label>Accrual Periodicity</rdfs:label>
<rdfs:comment>The frequency with which items are added to a collection.</rdfs:comment>
<dc:description>Recommended best practice is to use a value from a 
                 controlled vocabulary.</dc:description>
<rdfs:isDefinedBy rdf:resource="http://purl.org/dc/terms/"/>
<dcterms:issued>2005-06-13</dcterms:issued>
<dc:type rdf:resource="http://dublincore.org/usage/documents/principles/#element"/>
<dcterms:hasVersion rdf:resource="http://dublincore.org/usage/terms/history/#accrualPeriodicity-001"/>
</rdf:Property>
<rdf:Property rdf:about="http://purl.org/dc/terms/accrualPolicy">
<rdfs:label>Accrual Policy</rdfs:label>
<rdfs:comment>The policy governing the addition of items to a collection.</rdfs:comment>
<dc:description>Recommended best practice is to use a value from a controlled
                 vocabulary.</dc:description>
<rdfs:isDefinedBy rdf:resource="http://purl.org/dc/terms/"/>
<dcterms:issued>2005-06-13</dcterms:issued>
<dc:type rdf:resource="http://dublincore.org/usage/documents/principles/#element"/>
<dcterms:hasVersion rdf:resource="http://dublincore.org/usage/terms/history/#accrualPolicy-001"/>
</rdf:Property>
<rdfs:Class rdf:about="http://purl.org/dc/terms/SubjectScheme">
    <rdfs:label>Subject Encoding Schemes</rdfs:label>
    <rdfs:comment>A set of subject encoding schemes and/or formats</rdfs:comment>
    <rdfs:isDefinedBy rdf:resource="http://purl.org/dc/terms/"/>
    <dcterms:references rdf:resource="http://purl.org/dc/elements/1.1/subject"/>
    <dcterms:issued>2000-07-11</dcterms:issued>
  </rdfs:Class>
<rdfs:Class rdf:about="http://purl.org/dc/terms/DateScheme">
    <rdfs:label>Date Encoding Schemes</rdfs:label>
    <rdfs:comment>A set of date encoding schemes and/or formats </rdfs:comment>
    <dcterms:references rdf:resource="http://purl.org/dc/elements/1.1/date"/>
    <dcterms:references rdf:resource="http://purl.org/dc/terms/temporal"/>
    <rdfs:isDefinedBy rdf:resource="http://purl.org/dc/terms/"/>
    <dcterms:issued>2000-07-11</dcterms:issued>
  </rdfs:Class>
<rdfs:Class rdf:about="http://purl.org/dc/terms/FormatScheme">
    <rdfs:label>Format Encoding Schemes</rdfs:label>
    <rdfs:comment>A set of format encoding schemes.</rdfs:comment>
    <dcterms:references rdf:resource="http://purl.org/dc/elements/1.1/format"/>
    <rdfs:isDefinedBy rdf:resource="http://purl.org/dc/terms/"/>
    <dcterms:issued>2000-07-11</dcterms:issued>
  </rdfs:Class>
<rdfs:Class rdf:about="http://purl.org/dc/terms/LanguageScheme">
    <rdfs:label>Language Encoding Schemes</rdfs:label>
    <rdfs:comment>A set of language encoding schemes and/or formats.</rdfs:comment>
    <dcterms:references rdf:resource="http://purl.org/dc/elements/1.1/language"/>
    <rdfs:isDefinedBy rdf:resource="http://purl.org/dc/terms/"/>
    <dcterms:issued>2000-07-11</dcterms:issued>
  </rdfs:Class>
<rdfs:Class rdf:about="http://purl.org/dc/terms/SpatialScheme">
    <rdfs:label>Place Encoding Schemes</rdfs:label>
    <rdfs:comment>A set of geographic place encoding schemes and/or formats</rdfs:comment>
    <rdfs:isDefinedBy rdf:resource="http://purl.org/dc/terms/"/>
    <dcterms:references rdf:resource="http://purl.org/dc/terms/spatial"/>
    <dcterms:issued>2000-07-11</dcterms:issued>
  </rdfs:Class>
<rdfs:Class rdf:about="http://purl.org/dc/terms/TemporalScheme">
    <rdfs:label>Encoding Schemes
      for temporal characteristics</rdfs:label>
    <rdfs:comment>A set of encoding schemes for 
     the coverage qualifier "temporal"</rdfs:comment>
    <rdfs:isDefinedBy rdf:resource="http://purl.org/dc/terms/"/>
    <dcterms:issued>2000-07-11</dcterms:issued>
    <dcterms:references rdf:resource="http://purl.org/dc/terms/temporal"/>
  </rdfs:Class>
<rdfs:Class rdf:about="http://purl.org/dc/terms/TypeScheme">
    <rdfs:label>Resource Type Encoding Schemes</rdfs:label>
    <rdfs:comment>A set of resource type encoding schemes and/or formats</rdfs:comment>
    <rdfs:isDefinedBy rdf:resource="http://purl.org/dc/terms/"/>
    <dcterms:issued>2000-07-11</dcterms:issued>
    <dcterms:references rdf:resource="http://purl.org/dc/elements/1.1/type"/>
  </rdfs:Class>
<rdfs:Class rdf:about="http://purl.org/dc/terms/IdentifierScheme">
    <rdfs:label>Resource Identifier Encoding Schemes</rdfs:label>
    <rdfs:comment>A set of resource identifier encoding schemes and/or formats</rdfs:comment>
   <rdfs:isDefinedBy rdf:resource="http://purl.org/dc/terms/"/>
    <dcterms:issued>2000-07-11</dcterms:issued>
    <dcterms:references rdf:resource="http://purl.org/dc/elements/1.1/identifier"/>
  </rdfs:Class>
<rdfs:Class rdf:about="http://purl.org/dc/terms/RelationScheme">
    <rdfs:label>Resource Relation Encoding Schemes</rdfs:label>
    <rdfs:comment>A set of resource relation encoding schemes and/or formats</rdfs:comment>
    <rdfs:isDefinedBy rdf:resource="http://purl.org/dc/terms/"/>
    <dcterms:issued>2000-07-11</dcterms:issued>
    <dcterms:references rdf:resource="http://purl.org/dc/elements/1.1/relation"/>
  </rdfs:Class>
<rdfs:Class rdf:about="http://purl.org/dc/terms/SourceScheme">
    <rdfs:label>Source Encoding Schemes</rdfs:label>
    <rdfs:comment>A set of source encoding schemes and/or formats</rdfs:comment>
    <rdfs:isDefinedBy rdf:resource="http://purl.org/dc/terms/"/>
    <dcterms:issued>2000-07-11</dcterms:issued>
    <dcterms:references rdf:resource="http://purl.org/dc/elements/1.1/source"/>
  </rdfs:Class>
<dcterms:SubjectScheme rdf:about="http://purl.org/dc/terms/LCSH">
<rdfs:label>LCSH</rdfs:label>
<rdfs:comment>Library of Congress Subject Headings</rdfs:comment>
<rdf:type rdf:resource="http://www.w3.org/2000/01/rdf-schema#Class"/>
<rdfs:isDefinedBy rdf:resource="http://purl.org/dc/terms/"/>
<dcterms:issued>2000-07-11</dcterms:issued>
<dcterms:modified>2002-06-15</dcterms:modified>
<dc:type rdf:resource="http://dublincore.org/usage/documents/principles/#encoding-scheme"/>
<dcterms:hasVersion rdf:resource="http://dublincore.org/usage/terms/history/#LCSH-002"/>
</dcterms:SubjectScheme>
<dcterms:SubjectScheme rdf:about="http://purl.org/dc/terms/MESH">
<rdfs:label>MeSH</rdfs:label>
<rdfs:comment>Medical Subject Headings</rdfs:comment>
<rdf:type rdf:resource="http://www.w3.org/2000/01/rdf-schema#Class"/>
<rdfs:isDefinedBy rdf:resource="http://purl.org/dc/terms/"/>
<rdfs:seeAlso rdf:resource="http://www.nlm.nih.gov/mesh/meshhome.html"/>
<dcterms:issued>2000-07-11</dcterms:issued>
<dcterms:modified>2002-06-15</dcterms:modified>
<dc:type rdf:resource="http://dublincore.org/usage/documents/principles/#encoding-scheme"/>
<dcterms:hasVersion rdf:resource="http://dublincore.org/usage/terms/history/#MESH-002"/>
</dcterms:SubjectScheme>
<dcterms:SubjectScheme rdf:about="http://purl.org/dc/terms/DDC">
<rdfs:label>DDC</rdfs:label>
<rdfs:comment>Dewey Decimal Classification</rdfs:comment>
<rdf:type rdf:resource="http://www.w3.org/2000/01/rdf-schema#Class"/>
<rdfs:isDefinedBy rdf:resource="http://purl.org/dc/terms/"/>
<rdfs:seeAlso rdf:resource="http://www.oclc.org/dewey/"/>
<dcterms:issued>2000-07-11</dcterms:issued>
<dcterms:modified>2002-06-15</dcterms:modified>
<dc:type rdf:resource="http://dublincore.org/usage/documents/principles/#encoding-scheme"/>
<dcterms:hasVersion rdf:resource="http://dublincore.org/usage/terms/history/#DDC-002"/>
</dcterms:SubjectScheme>
<dcterms:SubjectScheme rdf:about="http://purl.org/dc/terms/LCC">
<rdfs:label>LCC</rdfs:label>
<rdfs:comment>Library of Congress Classification</rdfs:comment>
<rdf:type rdf:resource="http://www.w3.org/2000/01/rdf-schema#Class"/>
<rdfs:isDefinedBy rdf:resource="http://purl.org/dc/terms/"/>
<rdfs:seeAlso rdf:resource="http://lcweb.loc.gov/catdir/cpso/lcco/lcco.html"/>
<dcterms:issued>2000-07-11</dcterms:issued>
<dcterms:modified>2002-06-15</dcterms:modified>
<dc:type rdf:resource="http://dublincore.org/usage/documents/principles/#encoding-scheme"/>
<dcterms:hasVersion rdf:resource="http://dublincore.org/usage/terms/history/#LCC-002"/>
</dcterms:SubjectScheme>
<dcterms:SubjectScheme rdf:about="http://purl.org/dc/terms/UDC">
<rdfs:label>UDC</rdfs:label>
<rdfs:comment>Universal Decimal Classification</rdfs:comment>
<rdf:type rdf:resource="http://www.w3.org/2000/01/rdf-schema#Class"/>
<rdfs:isDefinedBy rdf:resource="http://purl.org/dc/terms/"/>
<rdfs:seeAlso rdf:resource="http://www.udcc.org/"/>
<dcterms:issued>2000-07-11</dcterms:issued>
<dcterms:modified>2002-06-15</dcterms:modified>
<dc:type rdf:resource="http://dublincore.org/usage/documents/principles/#encoding-scheme"/>
<dcterms:hasVersion rdf:resource="http://dublincore.org/usage/terms/history/#UDC-002"/>
</dcterms:SubjectScheme>
<dcterms:TypeScheme rdf:about="http://purl.org/dc/terms/DCMIType">
<rdfs:label>DCMI Type Vocabulary</rdfs:label>
<rdfs:comment>A list of types used to categorize the nature or genre 
										of the content of the resource.</rdfs:comment>
<rdf:type rdf:resource="http://www.w3.org/2000/01/rdf-schema#Class"/>
<rdfs:isDefinedBy rdf:resource="http://purl.org/dc/terms/"/>
<rdfs:seeAlso rdf:resource="http://dublincore.org/documents/dcmi-type-vocabulary/"/>
<dcterms:issued>2000-07-11</dcterms:issued>
<dcterms:modified>2002-06-15</dcterms:modified>
<dc:type rdf:resource="http://dublincore.org/usage/documents/principles/#encoding-scheme"/>
<dcterms:hasVersion rdf:resource="http://dublincore.org/usage/terms/history/#DCMIType-002"/>
</dcterms:TypeScheme>
<dcterms:FormatScheme rdf:about="http://purl.org/dc/terms/IMT">
<rdfs:label>IMT</rdfs:label>
<rdfs:comment>The Internet media type of the resource.</rdfs:comment>
<rdf:type rdf:resource="http://www.w3.org/2000/01/rdf-schema#Class"/>
<rdfs:isDefinedBy rdf:resource="http://purl.org/dc/terms/"/>
<rdfs:seeAlso rdf:resource="http://www.iana.org/assignments/media-types/"/>
<dcterms:issued>2000-07-11</dcterms:issued>
<dcterms:modified>2004-12-17</dcterms:modified>
<dc:type rdf:resource="http://dublincore.org/usage/documents/principles/#encoding-scheme"/>
<dcterms:hasVersion rdf:resource="http://dublincore.org/usage/terms/history/#IMT-003"/>
</dcterms:FormatScheme>
<dcterms:LanguageScheme rdf:about="http://purl.org/dc/terms/ISO639-2">
<rdfs:label>ISO 639-2</rdfs:label>
<rdfs:comment>ISO 639-2: Codes for the representation of names of languages.</rdfs:comment>
<rdf:type rdf:resource="http://www.w3.org/2000/01/rdf-schema#Class"/>
<rdfs:isDefinedBy rdf:resource="http://purl.org/dc/terms/"/>
<rdfs:seeAlso rdf:resource="http://lcweb.loc.gov/standards/iso639-2/langhome.html"/>
<dcterms:issued>2000-07-11</dcterms:issued>
<dcterms:modified>2002-06-15</dcterms:modified>
<dc:type rdf:resource="http://dublincore.org/usage/documents/principles/#encoding-scheme"/>
<dcterms:hasVersion rdf:resource="http://dublincore.org/usage/terms/history/#ISO639-2-002"/>
</dcterms:LanguageScheme>
<dcterms:LanguageScheme rdf:about="http://purl.org/dc/terms/RFC1766">
<rdfs:label>RFC 1766</rdfs:label>
<rdfs:comment>Internet RFC 1766 'Tags for the identification of Language' 
										specifies a two letter code taken from ISO 639, followed 
										optionally by a two letter country code taken from ISO 3166.</rdfs:comment>
<rdf:type rdf:resource="http://www.w3.org/2000/01/rdf-schema#Class"/>
<rdfs:isDefinedBy rdf:resource="http://purl.org/dc/terms/"/>
<rdfs:seeAlso rdf:resource="http://www.ietf.org/rfc/rfc1766.txt"/>
<dcterms:issued>2000-07-11</dcterms:issued>
<dcterms:modified>2002-06-15</dcterms:modified>
<dc:type rdf:resource="http://dublincore.org/usage/documents/principles/#encoding-scheme"/>
<dcterms:hasVersion rdf:resource="http://dublincore.org/usage/terms/history/#RFC1766-002"/>
</dcterms:LanguageScheme>
<dcterms:IdentifierScheme rdf:about="http://purl.org/dc/terms/URI">
<rdfs:label>URI</rdfs:label>
<rdfs:comment>A URI Uniform Resource Identifier</rdfs:comment>
<rdf:type rdf:resource="http://www.w3.org/2000/01/rdf-schema#Class"/>
<rdf:type rdf:resource="http://purl.org/dc/terms/SourceScheme"/>
<rdf:type rdf:resource="http://purl.org/dc/terms/RelationScheme"/>
<rdfs:isDefinedBy rdf:resource="http://purl.org/dc/terms/"/>
<rdfs:seeAlso rdf:resource="http://www.ietf.org/rfc/rfc2396.txt"/>
<dcterms:issued>2000-07-11</dcterms:issued>
<dcterms:modified>2002-06-15</dcterms:modified>
<dc:type rdf:resource="http://dublincore.org/usage/documents/principles/#encoding-scheme"/>
<dcterms:hasVersion rdf:resource="http://dublincore.org/usage/terms/history/#URI-002"/>
</dcterms:IdentifierScheme>
<dcterms:SpatialScheme rdf:about="http://purl.org/dc/terms/Point">
<rdfs:label>DCMI Point</rdfs:label>
<rdfs:comment>The DCMI Point identifies a point in space using its geographic coordinates.</rdfs:comment>
<rdf:type rdf:resource="http://www.w3.org/2000/01/rdf-schema#Class"/>
<rdfs:isDefinedBy rdf:resource="http://purl.org/dc/terms/"/>
<rdfs:seeAlso rdf:resource="http://dublincore.org/documents/dcmi-point/"/>
<dcterms:issued>2000-07-11</dcterms:issued>
<dcterms:modified>2002-06-15</dcterms:modified>
<dc:type rdf:resource="http://dublincore.org/usage/documents/principles/#encoding-scheme"/>
<dcterms:hasVersion rdf:resource="http://dublincore.org/usage/terms/history/#Point-002"/>
</dcterms:SpatialScheme>
<dcterms:SpatialScheme rdf:about="http://purl.org/dc/terms/ISO3166">
<rdfs:label>ISO 3166</rdfs:label>
<rdfs:comment>ISO 3166 Codes for the representation of names of countries</rdfs:comment>
<rdf:type rdf:resource="http://www.w3.org/2000/01/rdf-schema#Class"/>
<rdfs:isDefinedBy rdf:resource="http://purl.org/dc/terms/"/>
<rdfs:seeAlso rdf:resource="http://www.iso.org/iso/en/prods-services/iso3166ma/02iso-3166-code-lists/list-en1.html"/>
<dcterms:issued>2000-07-11</dcterms:issued>
<dcterms:modified>2004-12-17</dcterms:modified>
<dc:type rdf:resource="http://dublincore.org/usage/documents/principles/#encoding-scheme"/>
<dcterms:hasVersion rdf:resource="http://dublincore.org/usage/terms/history/#ISO3166-003"/>
</dcterms:SpatialScheme>
<dcterms:SpatialScheme rdf:about="http://purl.org/dc/terms/Box">
<rdfs:label>DCMI Box</rdfs:label>
<rdfs:comment>The DCMI Box identifies a region of space using its geographic limits.</rdfs:comment>
<rdf:type rdf:resource="http://www.w3.org/2000/01/rdf-schema#Class"/>
<rdfs:isDefinedBy rdf:resource="http://purl.org/dc/terms/"/>
<rdfs:seeAlso rdf:resource="http://dublincore.org/documents/dcmi-box/"/>
<dcterms:issued>2000-07-11</dcterms:issued>
<dcterms:modified>2002-06-15</dcterms:modified>
<dc:type rdf:resource="http://dublincore.org/usage/documents/principles/#encoding-scheme"/>
<dcterms:hasVersion rdf:resource="http://dublincore.org/usage/terms/history/#Box-002"/>
</dcterms:SpatialScheme>
<dcterms:SpatialScheme rdf:about="http://purl.org/dc/terms/TGN">
<rdfs:label>TGN</rdfs:label>
<rdfs:comment>The Getty Thesaurus of Geographic Names</rdfs:comment>
<rdf:type rdf:resource="http://www.w3.org/2000/01/rdf-schema#Class"/>
<rdfs:isDefinedBy rdf:resource="http://purl.org/dc/terms/"/>
<rdfs:seeAlso rdf:resource="http://www.getty.edu/research/tools/vocabulary/tgn/index.html"/>
<dcterms:issued>2000-07-11</dcterms:issued>
<dcterms:modified>2002-06-15</dcterms:modified>
<dc:type rdf:resource="http://dublincore.org/usage/documents/principles/#encoding-scheme"/>
<dcterms:hasVersion rdf:resource="http://dublincore.org/usage/terms/history/#TGN-002"/>
</dcterms:SpatialScheme>
<dcterms:DateScheme rdf:about="http://purl.org/dc/terms/Period">
<rdfs:label>DCMI Period</rdfs:label>
<rdfs:comment>A specification of the limits of a time interval.</rdfs:comment>
<rdf:type rdf:resource="http://www.w3.org/2000/01/rdf-schema#Class"/>
<rdf:type rdf:resource="http://purl.org/dc/terms/TemporalScheme"/>
<rdfs:isDefinedBy rdf:resource="http://purl.org/dc/terms/"/>
<rdfs:seeAlso rdf:resource="http://dublincore.org/documents/dcmi-period/"/>
<dcterms:issued>2000-07-11</dcterms:issued>
<dcterms:modified>2002-06-15</dcterms:modified>
<dc:type rdf:resource="http://dublincore.org/usage/documents/principles/#encoding-scheme"/>
<dcterms:hasVersion rdf:resource="http://dublincore.org/usage/terms/history/#Period-002"/>
</dcterms:DateScheme>
<dcterms:DateScheme rdf:about="http://purl.org/dc/terms/W3CDTF">
<rdfs:label>W3C-DTF</rdfs:label>
<rdfs:comment>W3C Encoding rules for dates and times - a profile based on ISO 8601</rdfs:comment>
<rdf:type rdf:resource="http://www.w3.org/2000/01/rdf-schema#Class"/>
<rdf:type rdf:resource="http://purl.org/dc/terms/TemporalScheme"/>
<rdfs:isDefinedBy rdf:resource="http://purl.org/dc/terms/"/>
<rdfs:seeAlso rdf:resource="http://www.w3.org/TR/NOTE-datetime"/>
<dcterms:issued>2000-07-11</dcterms:issued>
<dcterms:modified>2002-06-15</dcterms:modified>
<dc:type rdf:resource="http://dublincore.org/usage/documents/principles/#encoding-scheme"/>
<dcterms:hasVersion rdf:resource="http://dublincore.org/usage/terms/history/#W3CDTF-002"/>
</dcterms:DateScheme>
<dcterms:LanguageScheme rdf:about="http://purl.org/dc/terms/RFC3066">
<rdfs:label>RFC 3066</rdfs:label>
<rdfs:comment>Internet RFC 3066 'Tags for the Identification of 
		Languages' specifies a primary subtag which
		is a two-letter code taken from ISO 639 part
		1 or a three-letter code taken from ISO 639
		part 2, followed optionally by a two-letter
		country code taken from ISO 3166.  When a
		language in ISO 639 has both a two-letter and
		three-letter code, use the two-letter code;
		when it has only a three-letter code, use the
		three-letter code.  This RFC replaces RFC
		1766.</rdfs:comment>
<rdf:type rdf:resource="http://www.w3.org/2000/01/rdf-schema#Class"/>
<rdfs:isDefinedBy rdf:resource="http://purl.org/dc/terms/"/>
<rdfs:seeAlso rdf:resource="http://www.ietf.org/rfc/rfc3066.txt"/>
<dcterms:issued>2002-07-13</dcterms:issued>
<dc:type rdf:resource="http://dublincore.org/usage/documents/principles/#encoding-scheme"/>
<dcterms:hasVersion rdf:resource="http://dublincore.org/usage/terms/history/#RFC3066-001"/>
</dcterms:LanguageScheme>
<dcterms:SubjectScheme rdf:about="http://purl.org/dc/terms/NLM">
<rdfs:label>NLM</rdfs:label>
<rdfs:comment>National Library of Medicine Classification</rdfs:comment>
<rdf:type rdf:resource="http://www.w3.org/2000/01/rdf-schema#Class"/>
<rdfs:isDefinedBy rdf:resource="http://purl.org/dc/terms/"/>
<rdfs:seeAlso rdf:resource="http://wwwcf.nlm.nih.gov/class/"/>
<dcterms:issued>2005-06-13</dcterms:issued>
<dc:type rdf:resource="http://dublincore.org/usage/documents/principles/#encoding-scheme"/>
<dcterms:hasVersion rdf:resource="http://dublincore.org/usage/terms/history/#NLM-001"/>
</dcterms:SubjectScheme>
</rdf:RDF>
