<?xml version='1.0' encoding='UTF-8'?>
<!DOCTYPE rdf:RDF [
	 <!ENTITY nie 'http://ont.semanticdesktop.org/2007/01/nie#'>
	 <!ENTITY a 'http://protege.stanford.edu/system#'>
	 <!ENTITY rdfs 'http://www.w3.org/2000/01/rdf-schema#'>
	 <!ENTITY nfo_ 'http://ont.semanticdesktop.org/2007/03/22/nfo#'>
	 <!ENTITY xsd 'http://www.w3.org/2001/XMLSchema#'>
	 <!ENTITY nexif 'http://ont.semanticdesktop.org/2007/05/10/nexif#'>
	 <!ENTITY nmpeg7 'http://ont.semanticdesktop.org/2007/05/10/nmpeg7#'>
	 <!ENTITY nco 'http://ont.semanticdesktop.org/2007/03/22/nco#'>
	 <!ENTITY rdf 'http://www.w3.org/1999/02/22-rdf-syntax-ns#'>
	 <!ENTITY dc 'http://purl.org/dc/elements/1.1/'>
]>
<rdf:RDF xmlns:nie="&nie;"
	 xmlns:a="&a;"
	 xmlns:rdfs="&rdfs;"
	 xmlns:nfo_="&nfo_;"
	 xmlns:xsd="&xsd;"
	 xmlns:nexif="&nexif;"
	 xmlns:nmpeg7="&nmpeg7;"
	 xmlns:nco="&nco;"
	 xmlns:rdf="&rdf;"
	 xmlns:dc="&dc;">
<rdfs:Class rdf:about="&nfo_;CompressedFile"
	 rdfs:label="CompressedFile">
	<rdfs:comment>A compressed file. May contain other files or folder inside. </rdfs:comment>
	<rdfs:subClassOf rdf:resource="&nfo_;File"/>
	<rdfs:subClassOf rdf:resource="&nfo_;Folder"/>
</rdfs:Class>
<rdfs:Class rdf:about="&nfo_;ExecutableFile"
	 rdfs:comment="An executable file."
	 rdfs:label="ExecutableFile">
	<rdfs:subClassOf rdf:resource="&nfo_;File"/>
</rdfs:Class>
<rdfs:Class rdf:about="&nfo_;ExifFile"
	 rdfs:comment="An image file with Exif annotations."
	 rdfs:label="ExifFile">
	<rdfs:subClassOf rdf:resource="&nfo_;ImageFile"/>
	<rdfs:subClassOf rdf:resource="&nexif;IFD"/>
</rdfs:Class>
<rdfs:Class rdf:about="&nfo_;File"
	 rdfs:label="File">
	<rdfs:comment>A resource containing a finite sequence of bytes with arbitrary information, that is available to a computer program and is usually based on some kind of durable storage. A file is durable in the sense that it remains available for programs to use after the current program has finished.</rdfs:comment>
	<rdfs:subClassOf rdf:resource="&nie;DataObject"/>
</rdfs:Class>
<rdfs:Class rdf:about="&nfo_;FileHash"
	 rdfs:label="FileHash">
	<rdfs:comment>A fingerprint of the file, generated by some hashing function.</rdfs:comment>
	<rdfs:subClassOf rdf:resource="&rdfs;Resource"/>
</rdfs:Class>
<rdfs:Class rdf:about="&nfo_;Folder"
	 rdfs:comment="A folder/directory. May contain files or other folders."
	 rdfs:label="Folder">
	<rdfs:subClassOf rdf:resource="&nie;DataObject"/>
</rdfs:Class>
<rdfs:Class rdf:about="&nfo_;ImageFile"
	 rdfs:comment="A file containing an image."
	 rdfs:label="ImageFile">
	<rdfs:subClassOf rdf:resource="&nfo_;VisualFile"/>
</rdfs:Class>
<rdfs:Class rdf:about="&nfo_;MediaFileList"
	 rdfs:comment="A file containing a list of media files.e.g. a playlist"
	 rdfs:label="MediaFileList">
	<rdfs:subClassOf rdf:resource="&nfo_;File"/>
</rdfs:Class>
<rdfs:Class rdf:about="&nfo_;MediaFileListEntry"
	 rdfs:label="MediaFileListEntry">
	<rdfs:comment>A single node in the list of audio files contained within an AudioFileList instance. This class is intended to provide a type all those links have. In valid NRL untyped resources cannot be linked. There are no properties defined for this class but the application may expect rdf:first and rdf:last links. The former points to the AudioFile instance the latter points at another AuidoFileListEntry respectively. At the end of the list there is a link to rdf:nil.</rdfs:comment>
	<rdfs:subClassOf rdf:resource="&rdfs;Resource"/>
</rdfs:Class>
<rdfs:Class rdf:about="&nfo_;MindMap"
	 rdfs:label="MindMap">
	<rdfs:comment>A file containig a MindMap, created by a mind-mapping utility. Examples might include FreeMind or mind mapper.</rdfs:comment>
	<rdfs:subClassOf rdf:resource="&nfo_;File"/>
</rdfs:Class>
<rdfs:Class rdf:about="&nfo_;PaginatedTextDocument"
	 rdfs:label="PaginatedTextDocument">
	<rdfs:comment>A file containing a text document, that is unambiguously divided into pages. Examples might include PDF, DOC, PS, DVI etc.</rdfs:comment>
	<rdfs:subClassOf rdf:resource="&nfo_;TextDocument"/>
</rdfs:Class>
<rdfs:Class rdf:about="&nfo_;Presentation"
	 rdfs:label="Presentation">
	<rdfs:comment>A Presentation made by some presentation software (Corel Presentations, OpenOffice Impress, MS Powerpoint etc.)</rdfs:comment>
	<rdfs:subClassOf rdf:resource="&nfo_;File"/>
</rdfs:Class>
<rdfs:Class rdf:about="&nfo_;SourceCodeFile"
	 rdfs:label="SourceCodeFile">
	<rdfs:comment>A plain-text file containing code in a compilable or interpreted language.</rdfs:comment>
	<rdfs:subClassOf rdf:resource="&nfo_;File"/>
</rdfs:Class>
<rdfs:Class rdf:about="&nfo_;SpreadsheetFile"
	 rdfs:label="SpreadsheetFile">
	<rdfs:comment>A file containing a spreadsheet, created by a spreadsheet application. Examples might include Gnumeric, OpenOffice Calc or MS Excel.</rdfs:comment>
	<rdfs:subClassOf rdf:resource="&nfo_;File"/>
</rdfs:Class>
<rdfs:Class rdf:about="&nfo_;TextDocument"
	 rdfs:label="TextDocument">
	<rdfs:comment>A text document, either created with a word-processor (OpenOffice Writer, or MS Word) or a DTP application (e.g. a PDF, or PS).</rdfs:comment>
	<rdfs:subClassOf rdf:resource="&nfo_;File"/>
</rdfs:Class>
<rdfs:Class rdf:about="&nfo_;VideoFile"
	 rdfs:comment="A video file."
	 rdfs:label="VideoFile">
	<rdfs:subClassOf rdf:resource="&nfo_;VisualFile"/>
</rdfs:Class>
<rdfs:Class rdf:about="&nfo_;VisualFile"
	 rdfs:comment="File containing visual content."
	 rdfs:label="VisualFile">
	<rdfs:subClassOf rdf:resource="&nfo_;MediaFile"/>
</rdfs:Class>
<rdfs:Class rdf:about="&nfo_;WebResource"
	 rdfs:label="WebResource">
	<rdfs:comment>A resource downloaded from the Web. This class is intended to as a mark to be applied over all other types of files if they happen to have been downloaded from the Web.</rdfs:comment>
	<rdfs:subClassOf rdf:resource="&rdfs;Resource"/>
</rdfs:Class>
<rdf:Property rdf:about="&nfo_;belongsToFolder"
	 a:maxCardinality="1"
	 rdfs:label="belongsToFolder">
	<rdfs:comment>Models the containment relations between Files and Folders (or CompressedFiles).</rdfs:comment>
	<rdfs:subPropertyOf rdf:resource="&nie;isPartOf"/>
	<rdfs:domain rdf:resource="&nfo_;File"/>
	<rdfs:range rdf:resource="&nfo_;Folder"/>
</rdf:Property>
<rdf:Property rdf:about="&nfo_;fileCreated"
	 a:maxCardinality="1"
	 rdfs:comment="File creation date"
	 rdfs:label="fileCreated">
	<rdfs:subPropertyOf rdf:resource="&nie;created"/>
	<rdfs:domain rdf:resource="&nfo_;File"/>
	<rdfs:range rdf:resource="&xsd;dateTime"/>
</rdf:Property>
<rdf:Property rdf:about="&nfo_;fileLastAccessed"
	 a:maxCardinality="1"
	 rdfs:comment="Time when the file was last accessed."
	 rdfs:label="fileLastAccessed">
	<rdfs:domain rdf:resource="&nfo_;File"/>
	<rdfs:subPropertyOf rdf:resource="&dc;date"/>
	<rdfs:range rdf:resource="&xsd;dateTime"/>
</rdf:Property>
<rdf:Property rdf:about="&nfo_;fileLastModified"
	 rdfs:comment="last modification date"
	 rdfs:label="fileLastModified">
	<rdfs:domain rdf:resource="&nfo_;File"/>
	<rdfs:subPropertyOf rdf:resource="&dc;date"/>
	<rdfs:range rdf:resource="&xsd;dateTime"/>
</rdf:Property>
<rdf:Property rdf:about="&nfo_;fileOwner"
	 a:maxCardinality="1"
	 rdfs:label="fileOwner">
	<rdfs:comment>The owner of the file as defined by the file system access rights feature.</rdfs:comment>
	<rdfs:subPropertyOf rdf:resource="&nie;byteSize"/>
	<rdfs:range rdf:resource="&nco;Contact"/>
	<rdfs:domain rdf:resource="&nfo_;File"/>
</rdf:Property>
<rdf:Property rdf:about="&nfo_;fileSize"
	 a:maxCardinality="1"
	 rdfs:label="fileSize">
	<rdfs:comment>The size of the file in bytes. For compressed files it means the size of the packed file, not of the contents. For folders it means the aggregated size of all contained files and folders </rdfs:comment>
	<rdfs:subPropertyOf rdf:resource="&nie;byteSize"/>
	<rdfs:domain rdf:resource="&nfo_;File"/>
	<rdfs:subPropertyOf rdf:resource="&dc;date"/>
	<rdfs:range rdf:resource="&xsd;integer"/>
</rdf:Property>
<rdf:Property rdf:about="&nfo_;fileUrl"
	 rdfs:label="fileUrl">
	<rdfs:comment>URL of the file. It points at the location of the file. In cases where creating a simple file:// or http:// URL for a file is difficult (e.g. for files inside compressed archives) the applications are encouraged to use conventions defined by Apache Commons VFS Project at http://jakarta.apache.org/  commons/ vfs/ filesystems.html.</rdfs:comment>
	<rdfs:domain rdf:resource="&nfo_;File"/>
	<rdfs:range rdf:resource="&rdfs;Resource"/>
</rdf:Property>
<rdf:Property rdf:about="&nfo_;hasAudioCoding"
	 a:maxCardinality="1"
	 rdfs:comment="Links an AudioFile with nmpeg7:AudioCoding information"
	 rdfs:label="hasAudioCoding">
	<rdfs:range rdf:resource="&nmpeg7;AudioCoding"/>
</rdf:Property>
<rdf:Property rdf:about="&nfo_;hasHash"
	 a:maxCardinality="1"
	 rdfs:comment="Links the file with it's hash value."
	 rdfs:label="hasHash">
	<rdfs:domain rdf:resource="&nfo_;File"/>
	<rdfs:range rdf:resource="&nfo_;FileHash"/>
</rdf:Property>
<rdf:Property rdf:about="&nfo_;hasMediaFileListEntry"
	 a:maxCardinality="1"
	 rdfs:label="hasMediaFileListEntry">
	<rdfs:comment>This property is intended to point to an RDF list of MediaFiles.</rdfs:comment>
	<rdfs:domain rdf:resource="&nfo_;MediaFileList"/>
	<rdfs:range rdf:resource="&nfo_;MediaFileListEntry"/>
</rdf:Property>
<rdf:Property rdf:about="&nfo_;hasVisualCoding"
	 a:maxCardinality="1"
	 rdfs:label="hasVisualCoding">
	<rdfs:comment>Links the VisualFile with an nmpeg7: VisualCoding information.</rdfs:comment>
	<rdfs:domain rdf:resource="&nfo_;VisualFile"/>
	<rdfs:range rdf:resource="&nmpeg7;VisualCoding"/>
</rdf:Property>
<rdf:Property rdf:about="&nfo_;hashAlgorithm"
	 a:maxCardinality="1"
	 rdfs:label="hashAlgorithm">
	<rdfs:comment>Name of the algorithm used to compute the hash value. Examples might include CRC32, MD5, SHA, TTH etc.</rdfs:comment>
	<rdfs:domain rdf:resource="&nfo_;FileHash"/>
	<rdfs:range rdf:resource="&xsd;string"/>
</rdf:Property>
<rdf:Property rdf:about="&nfo_;hashValue"
	 a:maxCardinality="1"
	 rdfs:comment="The actual value of the hash."
	 rdfs:label="hashValue">
	<rdfs:domain rdf:resource="&nfo_;FileHash"/>
	<rdfs:range rdf:resource="&xsd;string"/>
</rdf:Property>
<rdf:Property rdf:about="&nfo_;pageCount"
	 a:maxCardinality="1"
	 rdfs:comment="Number of pages."
	 rdfs:label="pageCount">
	<rdfs:domain rdf:resource="&nfo_;PaginatedTextDocument"/>
	<rdfs:range rdf:resource="&xsd;integer"/>
</rdf:Property>
<rdf:Property rdf:about="&nfo_;programmingLanguage"
	 a:maxCardinality="1"
	 rdfs:label="programmingLanguage">
	<rdfs:comment>Indicates the name of the programming language this source code file is written in. Examples might include 'C', 'C++', 'Java' etc.</rdfs:comment>
	<rdfs:domain rdf:resource="&nfo_;SourceCodeFile"/>
	<rdfs:range rdf:resource="&xsd;string"/>
</rdf:Property>
<rdf:Property rdf:about="&nfo_;uncompressedSize"
	 a:maxCardinality="1"
	 rdfs:comment="Uncompressed size of the content of a compressed file."
	 rdfs:label="uncompressedSize">
	<rdfs:domain rdf:resource="&nfo_;CompressedFile"/>
	<rdfs:subPropertyOf rdf:resource="&dc;date"/>
	<rdfs:range rdf:resource="&xsd;integer"/>
</rdf:Property>
</rdf:RDF>
